Minor changes.

ref_impl/src/verifier/fstar_files/trigger_example.fst
@@ -24,28 +24,34 @@ let rec map f x = match x with
 | LNil -> LNil
 | LCons hd tl -> LCons (f hd) (map f tl)
 
-val length_append : x : list 'a -> y : list 'a -> Lemma (requires True) (ensures length x + length y = length (append x y)) [SMTPat (append x y)]
-let rec length_append x y = match x with
+val lemma_length_append : x : list 'a -> y : list 'a -> Lemma
+  (requires True)
+  (ensures length x + length y = length (append x y)) [SMTPat (append x y)]
+let rec lemma_length_append x y = match x with
 | LNil -> ()
-| LCons hd tl -> length_append tl y
+| LCons hd tl -> lemma_length_append tl y
 
-val filter_append : p : ('a -> bool) -> x : list 'a -> y : list 'a 
-  -> Lemma (requires True) (ensures (append (filter p x) (filter p y)) == (filter p (append x y)))
+val lemma_length_map : f : ('a -> 'b) -> x : list 'a -> Lemma 
+  (requires True) 
+  (ensures length x = length (map f x)) [SMTPat (map f x)]
+let rec lemma_length_map f x = match x with 
+| LNil -> ()
+| LCons hd tl -> lemma_length_map f tl
+
+val lemma_length_filter : 
+p : ('a -> bool) -> x : list 'a -> Lemma 
+  (requires True) 
+  (ensures length x >= length (filter p x)) [SMTPat (filter p x)]
+let rec lemma_length_filter p x = match x with
+| LNil -> ()
+| LCons hd tl -> lemma_length_filter p tl
+
+val filter_append : p : ('a -> bool) -> x : list 'a -> y : list 'a -> Lemma 
+  (requires True) 
+  (ensures (append (filter p x) (filter p y)) == (filter p (append x y))) [SMTPat (filter p (append x y))]
 let rec filter_append p x y = match x with 
 | LNil -> ()
 | LCons hd tl ->  filter_append p tl y
-
-val filtered_lists_are_smaller : 
-p : ('a -> bool) -> x : list 'a -> Lemma (requires True) (ensures length x >= length (filter p x)) [SMTPat (filter p x)]
-let rec filtered_lists_are_smaller p x = match x with
-| LNil -> ()
-| LCons hd tl -> filtered_lists_are_smaller p tl
-
-val map_preserves_length : f : ('a -> 'b) -> x : list 'a 
-  -> Lemma (requires True) (ensures length x = length (map f x)) [SMTPat (map f x)]
-let rec map_preserves_length f x = match x with 
-| LNil -> ()
-| LCons hd tl -> map_preserves_length f tl
 
 val positive_fun : x : list 'a -> Tot nat
 let positive_fun x = length x
@@ -53,6 +59,10 @@ let positive_fun x = length x
 val another_positive_fun : x : list nat -> Tot nat
 let another_positive_fun x = length x - (length (filter (fun (x : nat) -> x = 0) x))
 
+val hmm : p : ('a -> bool) -> x : list 'a -> y : list 'a -> Lemma 
+  (requires True)
+  (ensures (length (filter p (append x y))) == (length (filter p x)) + (length (filter p y)))
+let hmm _ _ _ = ()
 
 assume type t
 
@@ -65,24 +75,10 @@ assume val plus_associative: x:t -> y:t -> z:t -> Lemma
 
 irreducible let trigger (x:t) (y:t) = True
 
+// assume val plus_comm : x:t -> y:t -> Lemma (requires True) (ensures x + y == y + x) [SMTPat (x + y)]
+
 val test: x:t -> y:t -> z:t -> Lemma
   (requires forall (a:t) (b:t).{:pattern (trigger a b)} trigger a b /\ a + b == b + a)
   (ensures  (x + y) + z == (z + y) + x)
 let test x y z = cut (trigger z y /\ trigger x (z + y))
-
-
-// assume type t
-
-// assume val (+): t -> t -> t
-
-// assume val plus_associative: x:t -> y:t -> z:t -> Lemma
-//   (requires True)
-//   (ensures  (x + y) + z == x + (y + z))
-//   [SMTPat ((x + y) + z)]
-
-// irreducible let trigger (x:t) (y:t) = True
-
-// val test: x:t -> y:t -> z:t -> Lemma
-//   (requires forall (a:t) (b:t).{:pattern (trigger a b)} trigger a b /\ a + b == b + a)
-//   (ensures  (x + y) + z == (z + y) + x)
-// let test x y z = cut (trigger z y /\ trigger x (z + y))
+// let test x y z = cut (trigger z y); cut (trigger x (z + y))
